standardize ext_spec

bedrock2/src/bedrock2/FE310CSemantics.v
@@ -8,6 +8,8 @@ Require Import coqutil.Z.HexNotation.
 Import String List.ListNotations.
 Local Open Scope string_scope. Local Open Scope Z_scope. Local Open Scope list_scope.
 
+(** This file defines MMIO-only semantics. There is nothing FE310-specific here. *)
+
 Definition MMIOREAD : string := "MMIOREAD".
 Definition MMIOWRITE : string := "MMIOWRITE".
 
@@ -24,6 +26,35 @@ End parameters. Notation parameters := parameters.parameters.
 
 Section WithParameters.
   Context {p : parameters}.
+  Import Interface.map.
+
+  Local Notation bedrock2_trace := (list (parameters.mem * String.string * list parameters.word * (parameters.mem * list parameters.word))).
+
+  (* FIXME: this is a copypaste from [riscv.Platform.FE310ExtSpec.FE310_mmio] *)
+  Definition isMMIOAddr (addr:parameters.word) :=
+    Ox "00020000" <= word.unsigned addr < Ox "00022000" \/
+    Ox "10008000" <= word.unsigned addr < Ox "10010000" \/
+    Ox "10012000" <= word.unsigned addr < Ox "10013000" \/
+    Ox "10013000" <= word.unsigned addr < Ox "10014000".
+  (* FIXME: this is a copypaste from [riscv.Platform.FE310ExtSpec.FE310_mmio] *)
+  Definition isMMIOAligned (n : nat) (addr : parameters.word) :=
+    n = 4%nat /\ word.unsigned addr mod 4 = 0.
+
+  Definition ext_spec (t : bedrock2_trace) (mGive : parameters.mem) a (args: list parameters.word) (post:parameters.mem -> list parameters.word -> Prop) :=
+    if String.eqb "MMIOWRITE" a
+    then
+      exists addr val, 
+        args = [addr; val] /\
+        (mGive = Interface.map.empty /\ isMMIOAddr addr /\ word.unsigned addr mod 4 = 0) /\
+        post Interface.map.empty nil
+    else if String.eqb "MMIOREAD" a
+    then
+      exists addr,
+        args = [addr] /\
+        (mGive = Interface.map.empty /\ isMMIOAddr addr /\ word.unsigned addr mod 4 = 0) /\
+        forall val, post Interface.map.empty [val]
+    else False.
+
   Global Instance semantics_parameters  : Semantics.parameters :=
     {|
     syntax := StringNamesSyntax.make BasicCSyntax.StringNames_params;
@@ -35,24 +66,11 @@ Section WithParameters.
     mem := parameters.mem;
     locals := SortedListString.map _;
     funname_env := SortedListString.map;
-    ext_spec t m action args post :=
-      if string_dec action MMIOREAD then
-      match args with
-      | [addr] =>
-        ((Ox"10012000" <= word.unsigned addr < Ox"10013000") \/
-         (Ox"10024000" <= word.unsigned addr < Ox"10025000")  )
-        /\ forall v, post m [v]
-      | _ => False
-      end else
-      if string_dec action MMIOWRITE then
-      match args with
-      | [addr; val] =>
-        ((Ox"10012000" <= word.unsigned addr < Ox"10013000") \/
-         (Ox"10024000" <= word.unsigned addr < Ox"10025000")  )
-        /\ post m []
-      |  _ => False
-      end else False;
+    Semantics.ext_spec := ext_spec;
   |}.
+
+  Global Instance ext_spec_ok : ext_spec.ok _.
+  Admitted.
   
   Axiom TODO_andres_differential_memory_log : False.
   Global Instance ok : Semantics.parameters_ok semantics_parameters.
@@ -61,13 +79,6 @@ Section WithParameters.
     { cbv; auto. }
     { exact (SortedListString.ok _). }
     { exact SortedListString.ok. }
-    split.
-    { case TODO_andres_differential_memory_log. }
-    1,2:
-      cbv [ext_spec semantics_parameters]; intros;
-      cbv [Morphisms.Proper Morphisms.respectful Morphisms.pointwise_relation Basics.impl] in *;
-        repeat match goal with |- context [string_dec ?a ?b] => destruct (string_dec a b) end;
-        destruct args as [|? [|? [|]]]; intuition eauto.
   Qed.
   
   (* COPY-PASTE these *)
